proof/crefine/X64/IsolatedThreadAction.thy
@@ -14,11 +14,15 @@ context begin interpretation Arch .
 datatype tcb_state_regs =
   TCBStateRegs (tsrState : thread_state) (tsrContext : "MachineTypes.register \<Rightarrow> machine_word")
 
+definition get_tcb_state_regs_tcb :: "tcb \<Rightarrow> tcb_state_regs" where
+  "get_tcb_state_regs_tcb tcb \<equiv> TCBStateRegs (tcbState tcb) ((user_regs \<circ> atcbContextGet \<circ> tcbArch) tcb)"
+
 definition
   get_tcb_state_regs :: "kernel_object option \<Rightarrow> tcb_state_regs"
 where
- "get_tcb_state_regs oko \<equiv> case oko of
-    Some (KOTCB tcb) \<Rightarrow> TCBStateRegs (tcbState tcb) ((user_regs o atcbContextGet o tcbArch) tcb)"
+ "get_tcb_state_regs oko \<equiv> case oko of Some (KOTCB tcb) \<Rightarrow> get_tcb_state_regs_tcb tcb"
+
+lemmas get_tcb_state_regs_defs = get_tcb_state_regs_def get_tcb_state_regs_tcb_def
 
 definition
   put_tcb_state_regs_tcb :: "tcb_state_regs \<Rightarrow> tcb \<Rightarrow> tcb"
@@ -35,6 +39,8 @@ where
  "put_tcb_state_regs tsr oko = Some (KOTCB (put_tcb_state_regs_tcb tsr
     (case oko of
        Some (KOTCB tcb) \<Rightarrow> tcb | _ \<Rightarrow> makeObject)))"
+
+lemmas put_tcb_state_regs_defs = put_tcb_state_regs_def put_tcb_state_regs_tcb_def
 
 definition
  "partial_overwrite idx tcbs ps \<equiv>
@@ -85,9 +91,8 @@ lemma get_tcb_state_regs_partial_overwrite[simp]:
    get_tcb_state_regs (partial_overwrite idx tcbs f (idx x))
       = tcbs x"
   apply (simp add: partial_overwrite_def)
-  apply (simp add: put_tcb_state_regs_def
-                   get_tcb_state_regs_def
-                   put_tcb_state_regs_tcb_def
+  apply (simp add: put_tcb_state_regs_defs
+                   get_tcb_state_regs_defs
             split: tcb_state_regs.split)
   done
 
@@ -185,8 +190,7 @@ lemma partial_overwrite_get_tcb_state_regs:
                       split: if_split)
   apply clarsimp
   apply (drule_tac x=xa in spec)
-  apply (clarsimp simp: obj_at'_def projectKOs put_tcb_state_regs_def
-                        get_tcb_state_regs_def put_tcb_state_regs_tcb_def)
+  apply (clarsimp simp: obj_at'_def put_tcb_state_regs_defs get_tcb_state_regs_defs)
   apply (case_tac obj, simp)
   done
 
@@ -275,10 +279,9 @@ lemma map_to_ctes_partial_overwrite:
   apply (case_tac "x \<in> range idx")
    apply (clarsimp simp: put_tcb_state_regs_def)
    apply (drule_tac x=xa in spec)
-   apply (clarsimp simp: obj_at'_def projectKOs objBits_simps'
+   apply (clarsimp simp: obj_at'_def objBits_simps'
                    cong: if_cong)
-   apply (simp add: put_tcb_state_regs_def put_tcb_state_regs_tcb_def
-                    objBits_simps'
+   apply (simp add: put_tcb_state_regs_tcb_def objBits_simps'
               cong: if_cong option.case_cong)
    apply (case_tac obj, simp split: tcb_state_regs.split if_split)
   apply simp
@@ -287,10 +290,9 @@ lemma map_to_ctes_partial_overwrite:
   apply (case_tac "x && ~~ mask (objBitsKO (KOTCB undefined)) \<in> range idx")
    apply (clarsimp simp: put_tcb_state_regs_def)
    apply (drule_tac x=xa in spec)
-   apply (clarsimp simp: obj_at'_def projectKOs objBits_simps'
+   apply (clarsimp simp: obj_at'_def objBits_simps'
                    cong: if_cong)
-   apply (simp add: put_tcb_state_regs_def put_tcb_state_regs_tcb_def
-                    objBits_simps'
+   apply (simp add: put_tcb_state_regs_tcb_def objBits_simps'
               cong: if_cong option.case_cong)
    apply (case_tac obj, simp split: tcb_state_regs.split if_split)
    apply (intro impI allI)
@@ -642,11 +644,12 @@ lemma modify_not_fail[simp]:
 lemma setObject_assert_modify:
   "\<lbrakk> updateObject v = updateObject_default v; (1::machine_word) < 2 ^ objBits v;
      \<And>ko v'. projectKO_opt ko = Some (v'::'a) \<Longrightarrow> objBitsKO ko = objBits v \<rbrakk> \<Longrightarrow>
-   setObject p (v::'a::pspace_storable) s = (do
-     assert (obj_at' (\<lambda>_::'a. True) p s);
+   setObject p (v::'a::pspace_storable) = (do
+     state_assert (obj_at' (\<lambda>_::'a. True) p);
      modify (ksPSpace_update (\<lambda>ps. ps(p \<mapsto> injectKOS v)))
-   od) s"
-  apply (clarsimp simp: assert_def setObject_modify split: if_split)
+   od)"
+  apply (rule ext)
+  apply (clarsimp simp: state_assert_def exec_get assert_def setObject_modify bind_assoc split: if_split)
   apply (clarsimp simp: setObject_def updateObject_default_def exec_gets split_def bind_assoc)
   apply (clarsimp simp: assert_opt_def assert_def alignCheck_assert projectKO_def
                  split: option.splits if_splits)
@@ -916,6 +919,20 @@ lemma oblivious_setVMRoot_schact:
                       split: if_split capability.split arch_capability.split option.split)+
 
 
+lemma oblivious_switchLocalFpuOwner_schact:
+  "oblivious (ksSchedulerAction_update f) (switchLocalFpuOwner new_owner)"
+  apply (simp add: switchLocalFpuOwner_def)
+  by (safe intro!: oblivious_bind
+      | simp_all add: fpuOwner_asrt_def saveFpuState_def loadFpuState_def asUser_def
+                      threadGet_def liftM_def threadSet_def
+               split: option.split)+
+
+lemma oblivious_lazyFpuRestore_schact:
+  "oblivious (ksSchedulerAction_update f) (lazyFpuRestore t)"
+  apply (simp add: lazyFpuRestore_def)
+  by (safe intro!: oblivious_bind
+      | simp_all add: threadGet_def liftM_def oblivious_switchLocalFpuOwner_schact)+
+
 lemma oblivious_switchToThread_schact:
   "oblivious (ksSchedulerAction_update f) (ThreadDecls_H.switchToThread t)"
   apply (simp add: Thread_H.switchToThread_def switchToThread_def bind_assoc
@@ -923,8 +940,8 @@ lemma oblivious_switchToThread_schact:
                    threadSet_def tcbSchedEnqueue_def unless_when asUser_def
                    getQueue_def setQueue_def storeWordUser_def setRegister_def
                    pointerInUserData_def isRunnable_def isStopped_def
-                   getThreadState_def tcbSchedDequeue_def tcbQueueRemove_def bitmap_fun_defs
-                   ksReadyQueues_asrt_def)
+                   getThreadState_def tcbSchedDequeue_def bitmap_fun_defs
+                   tcbQueueRemove_def ksReadyQueues_asrt_def)
   by (safe intro!: oblivious_bind
               | simp_all add: ready_qs_runnable_def idleThreadNotQueued_def
                               oblivious_setVMRoot_schact)+
@@ -1128,14 +1145,13 @@ lemma setCTE_isolatable:
     apply (rule ext)
     apply (clarsimp simp: partial_overwrite_get_tcb_state_regs
                    split: if_split)
-    apply (clarsimp simp: projectKOs get_tcb_state_regs_def
-                          put_tcb_state_regs_def put_tcb_state_regs_tcb_def
+    apply (clarsimp simp: get_tcb_state_regs_defs put_tcb_state_regs_defs
                           partial_overwrite_def
                    split: tcb_state_regs.split)
     apply (case_tac obj, simp add: projectKO_opt_tcb)
     apply (simp add: tcb_cte_cases_def split: if_split_asm)
    apply (drule_tac x=x in spec)
-   apply (clarsimp simp: obj_at'_def projectKOs objBits_simps subtract_mask(2) [symmetric])
+   apply (clarsimp simp: obj_at'_def objBits_simps subtract_mask(2) [symmetric])
    apply (erule notE[rotated], erule (3) tcb_ctes_clear[rotated])
   apply (simp add: select_f_returns select_f_asserts split: if_split)
   apply (intro conjI impI)
@@ -1211,8 +1227,7 @@ lemma isolate_thread_actions_threadSet_tcbState:
                 intro!: kernel_state.fold_congs[OF refl refl])
   apply (simp add: partial_overwrite_fun_upd
                    partial_overwrite_get_tcb_state_regs)
-  apply (clarsimp simp: put_tcb_state_regs_def put_tcb_state_regs_tcb_def
-                        projectKOs get_tcb_state_regs_def
+  apply (clarsimp simp: put_tcb_state_regs_defs get_tcb_state_regs_defs
                  elim!: obj_atE')
   apply (case_tac ko)
   apply (simp add: projectKO_opt_tcb)
@@ -1241,7 +1256,7 @@ lemma switchToThread_rewrite:
        (switchToThread t)
        (do Arch.switchToThread t; setCurThread t od)"
   apply (simp add: switchToThread_def Thread_H.switchToThread_def)
-  apply (monadic_rewrite_l tcbSchedDequeue_rewrite, simp)
+  apply (monadic_rewrite_l tcbSchedDequeue_rewrite \<open>wpsimp simp: o_def\<close>, simp)
    (* strip LHS of getters and asserts until LHS and RHS are the same *)
    apply (repeat_unless \<open>rule monadic_rewrite_refl\<close> monadic_rewrite_symb_exec_l)
       apply wpsimp+
@@ -1390,12 +1405,11 @@ lemma set_register_isolate:
                         partial_overwrite_fun_upd
                         partial_overwrite_get_tcb_state_regs)
   apply (drule_tac x=y in spec)
-  apply (clarsimp simp: obj_at'_def projectKOs objBits_simps
+  apply (clarsimp simp: obj_at'_def objBits_simps
                   cong: if_cong)
   apply (case_tac obj)
-  apply (simp add: projectKO_opt_tcb put_tcb_state_regs_def
-                   put_tcb_state_regs_tcb_def get_tcb_state_regs_def
-                   atcbContextGet_def
+  apply (simp add: projectKO_opt_tcb put_tcb_state_regs_defs
+                   get_tcb_state_regs_defs atcbContextGet_def
              cong: if_cong)
   done
 
@@ -1423,12 +1437,11 @@ lemma copy_register_isolate:
                         partial_overwrite_fun_upd
                         partial_overwrite_get_tcb_state_regs)
   apply (frule_tac x=x in spec, drule_tac x=y in spec)
-  apply (clarsimp simp: obj_at'_def projectKOs objBits_simps
+  apply (clarsimp simp: obj_at'_def objBits_simps
                   cong: if_cong)
   apply (case_tac obj, case_tac obja)
-  apply (simp add: projectKO_opt_tcb put_tcb_state_regs_def
-                   put_tcb_state_regs_tcb_def get_tcb_state_regs_def
-                   atcbContextGet_def
+  apply (simp add: projectKO_opt_tcb put_tcb_state_regs_defs
+                   get_tcb_state_regs_defs atcbContextGet_def
              cong: if_cong)
   apply (auto simp: fun_eq_iff split: if_split)
   done
