proof/crefine/X64/TcbAcc_C.thy
@@ -251,6 +251,33 @@ lemma sanitiseRegister_spec:
   apply (case_tac r; simp add: C_register_defs sanitiseRegister_def sanitiseOrFlags_def sanitiseAndFlags_def) (* long *)
   by word_bitwise
 
+lemma rf_sr_ksArchState_armHSCurFPU:
+  "(s, s') \<in> rf_sr \<Longrightarrow> cur_fpu_relation (armKSCurFPUOwner (ksArchState s)) (ksCurFPUOwner_' (globals s'))"
+  by (clarsimp simp: rf_sr_def cstate_relation_def carch_state_relation_def Let_def)
+
+lemma ccorres_pre_getCurFPUOwner:
+  assumes cc: "\<And>rv. ccorres r xf (P rv) (P' rv) hs (f rv) c"
+  shows
+    "ccorres r xf
+       (\<lambda>s. (\<forall>rv. (armKSCurFPUOwner \<circ> ksArchState) s = rv \<longrightarrow> P rv s))
+       {s. \<forall>rv fpu'. ksCurFPUOwner_' (globals s) = fpu' \<and> cur_fpu_relation rv fpu' \<longrightarrow> s \<in> P' rv} hs
+       (gets (armKSCurFPUOwner \<circ> ksArchState) >>= (\<lambda>rv. f rv)) c"
+  apply (rule ccorres_guard_imp)
+    apply (rule ccorres_symb_exec_l)
+       defer
+       apply wp[1]
+      apply (rule gets_sp)
+     apply (clarsimp simp: empty_fail_def simpler_gets_def)
+    apply assumption
+   apply clarsimp
+   defer
+   apply (rule ccorres_guard_imp)
+     apply (rule cc)
+    apply clarsimp
+   apply assumption
+  apply (simp add: rf_sr_ksArchState_armHSCurFPU)
+  done
+
 lemma getObject_tcb_wp':
   "\<lbrace>\<lambda>s. \<forall>t. ko_at' (t :: tcb) p s \<longrightarrow> Q t s\<rbrace> getObject p \<lbrace>Q\<rbrace>"
   by (clarsimp simp: getObject_def valid_def in_monad
